defined regsdata, changed CData and VT accordingly

rocq/RegsData.v
@@ -6,9 +6,11 @@ Import ListNotations.
 
 (* Arrays *)
 Module Array.
-  Definition t (A : Type) := list A.
+  Definition t (A : Type) : Type := list A.
 
   (* Operations *)
+
+  Definition length {A} (a: t A) : nat := length a.
 
   Fixpoint make {A} (n : nat) (init : A) : t A :=
     match n with
@@ -25,6 +27,9 @@ Module Array.
     | _ :: xs, 0 => x :: xs
     | y :: xs, S i' => y :: set xs i' x
     end.
+
+  Definition zipWith {A} {B} {C} (a : t A) (b: t B) (f : (A * B) -> C) : t C :=
+    map f (combine a b).
 
   (* Properties *)
 
@@ -97,20 +102,115 @@ End Array.
 
 (* Regsdata *)
 Module RegsData : CDATA.
-  Definition t : Set := nat.
+  Definition val : Type := option nat.
+  
+  Inductive t' : Type :=
+  | Complete (a_cp: Array.t val) (a_clk: Array.t val)
+  | Incomplete (l: list (nat * val * val)).
 
+  Definition t := t'.
   Definition p : Set := nat.
 
-  Definition compress (p: p) (t1: t) (t2: t): t := t1 + t2.
+  Definition is_valid_index (p: p) (i: nat) : Prop :=
+    0 <= i /\ i < p.
 
-  Definition is_valid (t: t) := True.
+  Definition get_index (e: nat * val * val) : nat :=
+    match e with
+    | (i, _, _ ) => i
+    end.
+
+  Definition is_valid (p: p) (t: t) : Prop :=
+    match t with
+    | Complete a_cp a_clk =>
+        Array.length a_cp = p /\ Array.length a_clk = p
+    | Incomplete l =>
+        length l < p /\ Forall (fun x => is_valid_index p (get_index x)) l
+    end.
+
+  (* a1 is older than a2 -> overwrite a1 with a2 
+   don't overwrite if a2 element is None *)
+  Definition merge_arrays (a1 a2 : Array.t val) : Array.t val :=
+    Array.zipWith a1 a2 (fun x =>
+                           match x with
+                           | (x1, None) => x1
+                           | (_, Some v) => Some v
+                           end).
+
+  (* list is more recent than arrays
+     closer to start of list => more recent 
+     -> should add elements at the end of the list first, so that they can be overwritten later 
+     don't overwrite if list element is None
+   *)
+  Fixpoint add_list_to_arrays (l: list (nat * val * val))
+    (a_cp: Array.t val) (a_clk: Array.t val) : (Array.t val) * (Array.t val) :=
+    match l with
+    | [] => (a_cp, a_clk)
+    | (i, cp, clk) :: l' =>
+        let (a_cp', a_clk') := add_list_to_arrays l' a_cp a_clk in
+        match cp, clk with
+        | None, None => (a_cp', a_clk')
+        | Some v_cp, None => (Array.set a_cp' i cp, a_clk')
+        | None, Some v_clk => (a_cp', Array.set a_clk' i clk)
+        | Some v_cp, Some v_clk => (Array.set a_cp i cp, Array.set a_clk i clk)
+        end
+    end.
+
+  (* array is more recent than list
+   only add list elem if what what there before is None *)
+  Fixpoint add_arrays_to_list (l: list (nat * val * val))
+    (a_cp: Array.t val) (a_clk: Array.t val) : (Array.t val) * (Array.t val) :=
+    match l with
+    | [] => (a_cp, a_clk)
+    | (i, cp, clk) :: l' =>
+        (* add cp clk to arrays if what is already there is None *)
+        let (a_cp', a_clk') :=
+          match Array.get a_cp i, Array.get a_clk i with
+          | Some None, Some None => (Array.set a_cp i cp, Array.set a_clk i clk)
+          | Some None, _ => (Array.set a_cp i cp, a_clk)
+          | _, Some None => (a_cp, Array.set a_clk i clk)
+          | _, _ => (a_cp, a_clk)
+          end in
+        (* then recursively call *)
+        add_arrays_to_list l' a_cp' a_clk'
+    end.
+
+  (* t1 is old, t2 is recent *)
+  Definition compress (p: p) (t1: t) (t2: t): t :=
+    match t1, t2 with
+    | Complete a_cp1 a_clk1, Complete a_cp2 a_clk2 =>
+        Complete (merge_arrays a_cp1 a_cp2) (merge_arrays a_clk1 a_clk2)
+    | Complete a_cp1 a_clk1, Incomplete l2 =>
+        let (a_cp, a_clk) := add_list_to_arrays l2 a_cp1 a_clk1 in
+        Complete a_cp a_clk
+    | Incomplete l1, Complete a_cp2 a_clk2 =>
+        let (a_cp, a_clk) := add_arrays_to_list l1 a_cp2 a_clk2 in
+        Complete a_cp a_clk
+    | Incomplete l1, Incomplete l2 =>
+        let l := l2 ++ l1 in
+        if Nat.leb (length l) p
+        then
+          let (a_cp, a_clk) := add_list_to_arrays l (Array.make p None) (Array.make p None) in
+          Complete a_cp a_clk
+        else Incomplete l
+    end.
+
+  Lemma merge_arrays_assoc : forall x y z,
+      merge_arrays x (merge_arrays y z) = merge_arrays (merge_arrays x y) z.
+  Proof.
+    intros x y z.
+    unfold merge_arrays.
+  Admitted.
 
   Lemma compress_assoc : forall x y z p,
       compress p x (compress p y z) = compress p (compress p x y) z.
-  Proof. 
-    intros. simpl.
-    unfold compress. lia.
-  Qed.
+  Proof.
+    intros x y z p.
+    destruct x as [cpx clkx | lx], y as [cpy clky | ly], z as [cpz clkz | lz].
+    - simpl.
+      repeat rewrite merge_arrays_assoc.
+      reflexivity.
+    - (* might do a function for single array and separate *)
+  Admitted.
   
 End RegsData.
 
